extraction/kcalls: use concrete arguments for shmem/bid/tid, which get specialized during extaction

src/examples/Kuiper.Mul.fst
@@ -16,19 +16,17 @@ fn kf (#size : erased nat{size > 0}) (* do NOT use erased pos, inference suffers
   (a1 a2 ar : gpu_array u64 size)
   (s1 s2 : erased (seq u64))
   (#_ : squash (len s1 == size /\ len s2 == size))
-  (ebid : enatlt size)
+  (bid : szlt size)
   preserves
-    gpu ** block_id size ebid **
+    gpu ** block_id size bid **
     pts_to a1 #(1.0R /. size) s1 **
     pts_to a2 #(1.0R /. size) s2 **
     emp
   requires
-    gpu_pts_to_slice ar ebid (ebid + 1) 's
+    gpu_pts_to_slice ar bid (bid + 1) 's
   ensures
-    gpu_pts_to_slice ar ebid (ebid + 1) seq![(smul s1 s2).[ebid]]
+    gpu_pts_to_slice ar bid (bid + 1) seq![(smul s1 s2).[bid]]
 {
-  let bid = get_bid ();
-  rewrite each ebid as SZ.v bid;
   assert (pure (bid >= 0));
   assert (pure (bid < size));
   let v1 = gpu_array_read #_ #_ #0 #size a1 bid;
@@ -36,7 +34,6 @@ fn kf (#size : erased nat{size > 0}) (* do NOT use erased pos, inference suffers
   let v = FStar.UInt64.(v1 *%^ v2);
   gpu_array_write #_ #_ #bid #(bid + 1) ar bid v;
   (**)with sr. assert gpu_pts_to_slice ar bid (bid + 1) sr;
-  (**)Seq.lemma_eq_intro sr seq![(smul s1 s2).[ebid]];
-  rewrite each SZ.v bid as ebid;
+  (**)Seq.lemma_eq_intro sr seq![(smul s1 s2).[bid]];
   ()
 }
