src/lib/kuiper/Kuiper.SizeT.fsti
@@ -12,6 +12,10 @@ module U64 = FStar.UInt64
 unfold type sz  = FStar.SizeT.t
 unfold type szp = x:sz{FStar.SizeT.v x > 0}
 unfold type szlt (n:nat) = i:sz{SZ.v i < n}
+unfold type szlt2
+  (b1 : SZ.t)
+  (b2 : SZ.t{SZ.fits (SZ.v b1 * SZ.v b2)}) = szlt (SZ.v (b1 `SZ.mul` b2))
+
 unfold type szpmultiple (k:pos) = x:szp{k /? SZ.v x}
 
 (* Throughout this repo we assume a 64bit machine. This
